{
 "metadata": {
  "name": "11-Cauchy-Euler Equations"
 },
 "nbformat": 3,
 "nbformat_minor": 0,
 "worksheets": [
  {
   "cells": [
    {
     "cell_type": "markdown",
     "metadata": {},
     "source": [
      "# 4.7 Cauchy-Euler Equations - Math 201\n",
      "### Dr. Florin Diacu (http://www.math.uvic.ca/faculty/diacu/)"
     ]
    },
    {
     "cell_type": "markdown",
     "metadata": {},
     "source": [
      "## Problem Of the Form\n",
      "$$ a_nx^n \\frac{d^ny}{dx^n} + a_{n-1}x^{n-1} \\frac{d^{n-1}}{dx^{n-1}}+...+a_1x\\frac{dy}{dx}+a_0y=g(x) $$\n",
      "Note the non-constant coefficients (depending on x)\n",
      "\n",
      "The idea is to **always check the form** $y(x)=x^m$ in the homogenious equation.\n",
      "To solve the non-homogenious you can use variation of parameters or undetermined coefficients.\n",
      "\n",
      "**We must assume that x is not zero, so we restrict ourselves from 0 to infinity.**"
     ]
    },
    {
     "cell_type": "markdown",
     "metadata": {},
     "source": [
      "## Second Order Case\n",
      "$$ ax^2y\\prime\\prime + bxy\\prime + cy = g(x) $$\n",
      "\n",
      "We're first interested in the homogenious equation:\n",
      "$$ ax^2y\\prime\\prime + bxy\\prime + cy = 0 $$\n",
      "(Once this is solved we'll use variation of parameters or undetermined coefficients.)\n",
      "\n",
      "$$ y(x) = x^m $$\n",
      "$$ y\\prime(x) = mx^{m-1} $$\n",
      "$$ y\\prime\\prime(x)= m(m-1)x^{m-2} $$\n",
      "\n",
      "Bringing this into the equation:\n",
      "$$ ax^2m(m-1)x^{m-2}+bxmx^{m-1}+cx^m = 0 $$\n",
      "$$ am(m-1)x^m + bmx^m + cx^m = 0 $$\n",
      "\n",
      "Dividing by $x^m, x\\in(0,\\infty)$:\n",
      "$$ am(m-1)+bm+c=0 $$\n",
      "$$ am^2+(b-a)m+c = 0 $$\n",
      "\n",
      "There are **three cases**:"
     ]
    },
    {
     "cell_type": "markdown",
     "metadata": {},
     "source": [
      "### Distinct Real Roots\n",
      "$m_1, m_2$ roots, $m_1\\neq m_2$.\n",
      "$$ y_1(x)=x^{m_1}, y_2(x)=x^{m_2} $$\n",
      "\n",
      "This is linearly independant.\n",
      "So the general solution of the homogenious equation:\n",
      "$$ y_c(x)=c_1x^{m_1}+c_2x^{m_2} $$\n",
      "\n",
      "**Ex.**\n",
      "$$ x^2y\\prime\\prime-2xy\\prime-4y=0 $$\n",
      "\n",
      "$$ y(x)=x^m $$\n",
      "$$ y\\prime(x)=mx^{m-1} $$\n",
      "$$ y\\prime\\prime(x)=m(m-1)x^{m-2} $$\n",
      "\n",
      "$$ x^2m(m-1)x^{m-2}-2xmx^{m-1}-4x^m = 0 $$\n",
      "$$ (m^2-3m-4)x^m = 0 $$\n",
      "Dividing by $x^m$:\n",
      "$$ (m^2-3m-4)=0 $$\n",
      "Factoring:\n",
      "$$ m_1= -1, m_2=4 $$\n",
      "\n",
      "Therefore:\n",
      "$$ y(x)=c_1x^{-1}+c_2x^4 $$"
     ]
    },
    {
     "cell_type": "markdown",
     "metadata": {},
     "source": [
      "### Real, Repeated Roots\n",
      "$$ m_1=m_2 \\in \\mathbb{R} $$\n",
      "$$ y_1{x}=x^{m_1} $$\n",
      "(From the quadratic equation)\n",
      "$$ m_1 = \\frac{a-b}{2a} $$\n",
      "To find a second linearly independant solution, use reduction (4.2)... in other words check a solution of the form:\n",
      "$$ y_2(x)=u(x)x^{m_1} $$\n",
      "\n",
      "After dividing by $ax^2$:\n",
      "$$ y\\prime\\prime+\\frac{b}{ax}y\\prime + \\frac{c}{ax^2}y = 0 $$\n",
      "\n",
      "*Recall*: $ y\\prime\\prime+ P(x)y\\prime + Q(x)y = 0 $\n",
      "$$ y_2(x)=y_1(x)\\int{\\frac{e^{-\\int{P(x)dx}}}{y_1^2(x)}}dx $$\n",
      "\n",
      "So, $P(x)=\\frac{b}{ax}$\n",
      "$$ \\int{P(X)dx}=\\frac{b}{a}\\ln{|x|} $$\n",
      "$$ y_2(x)=x^{m_1}\\int{\\frac{e^{-\\frac{b}{a}\\ln{|x|}}}{x^{2m_1}}}dx $$\n",
      "Simplifying:\n",
      "$$ y_2(x)=x^{m_1}\\int{x^{-\\frac{b}{a}}x^{-2m_1}}dx $$\n",
      "$$ y_2(x)= x^{m_1}=\\int{x^{-\\frac{b}{a}}x^{\\frac{b-a}{a}}}dx $$\n",
      "$$ y_2(x)=x^{m_1}=\\int{\\frac{dx}{x}}=x^{m_1}\\ln{x} $$General Solution:\n",
      "$$ y(x)=c_1x^{m_1}+c_2x^{m_1}\\ln{|x|} $$\n",
      "\n",
      "**Ex.**\n",
      "$$ 4x^2y\\prime\\prime + 8xy\\prime + y = 0 $$\n",
      "$$ y(x)=x^m $$\n",
      "$$ y\\prime(x)=mx^{m-1} $$\n",
      "$$ y\\prime\\prime(x)=m(m-1)x^{m-2} $$\n",
      "$$ x^m(4m^2+4m+1)=0 $$\n",
      "$$ m_1=m_2=-\\frac{1}{2} $$\n",
      "$$ y(x)=c_1x^{-\\frac{1}{2}}+c_2x^{-\\frac{1}{2}} \\ln{x} $$\n",
      "\n",
      "For higher orders we obtain linearly independent solutions:\n",
      "$$ x^{m_1}, x^{m_1}\\ln{x}, x^{m_1}(\\ln{x})^2, ... , x^{m_1}(\\ln{x})^{k-1} $$"
     ]
    },
    {
     "cell_type": "markdown",
     "metadata": {},
     "source": [
      "### Complex Conjugate Roots\n",
      "$$ m_1= \\alpha+i\\beta $$\n",
      "$$ m_2 = \\alpha-i\\beta $$\n",
      "$$ \\alpha, \\beta \\in \\mathbb{R}, \\beta > 0 $$\n",
      "\n",
      "$$ y(x)=c_1x^{\\alpha+i\\beta} + c_2x^{\\alpha-i\\beta} $$\n",
      "But these are complex. To obtain real solutions,\n",
      "$$ x^{i\\beta} = (e^{\\ln{x}})^{i\\beta} = e^{i\\beta\\ln{x}} $$\n",
      "\n",
      "Using Eulers formula:\n",
      "$$ x^{i\\beta} = \\cos{(\\beta\\ln{x})}+i\\sin{(\\beta\\ln{x})} $$\n",
      "Similarily:\n",
      "$$ x^{-i\\beta} = \\cos{(\\beta\\ln{x})}-i\\sin{(\\beta\\ln{x})} $$\n",
      "Noting:\n",
      "$$ x^{i\\beta} + x^{-i\\beta} = 2\\cos{(\\beta\\ln{x})} $$\n",
      "$$ x^{i\\beta}-x^{-i\\beta} = 2i\\sin{(\\beta\\ln{x})} $$\n",
      "\n",
      "Take $ c_1=c_2=1 $:\n",
      "$$ y_1=x^\\alpha(x^{i\\beta}+x^{i\\beta}) $$\n",
      "\n",
      "Take $$ c_1=1, c_2 = -1 $$\n",
      "$$ y_2=x^\\alpha(x^{i\\beta}-x^{-i\\beta})=2ix^\\alpha \\sin{(\\beta \\ln{x})} $$\n",
      "\n",
      "Checking for independence:\n",
      "$$ W(x^\\alpha\\cos{(\\beta\\ln{x})}, x^\\alpha\\sin{(\\beta\\ln{x})}) = \\beta x^{2\\alpha-1} \\neq 0 $$\n",
      "\n",
      "General Solution **memorize**:\n",
      "$$ y(x)=c_1x^\\alpha \\cos{(\\beta\\ln{x})}+c_2x^\\alpha \\sin{(\\beta \\ln{x})} $$\n",
      "\n",
      "**Ex.**\n",
      "$$ 4x^2y\\prime\\prime + 17y = 0 $$\n",
      "$$ y(1)=-1 $$\n",
      "$$ y\\prime(1) = - \\frac{1}{2} $$\n",
      "\n",
      "$$ y(x)=x^m $$\n",
      "$$ 4x^2y\\prime\\prime + 17y = x^m (4m(m-1)+17) = 0 $$\n",
      "$$ 4m^2-4m+17 = 0 $$\n",
      "$$ m_1 = \\frac{1}{2}+2i, m_2 = \\frac{1}{2}-2i $$\n",
      "$$ \\alpha = \\frac{1}{2}, \\beta = 2 $$\n",
      "\n",
      "From general solution:\n",
      "$$ y(x)=x^{\\frac{1}{2}}(c_1\\cos{(2\\ln{x})}+c_2\\sin{(2\\ln{x})} $$\n",
      "\n",
      "But this is an IVP:\n",
      "$$ -1 = y(1) = 1(c_1) $$\n",
      "\n",
      "$$ y\\prime(x)= \\frac{1}{2}x^{-\\frac{1}{2}}(c_1\\cos{(2\\ln{x})}+c_2\\sin{(2\\ln{x})} + x^{\\frac{1}{2}}(-c_1\\sin{(2\\ln{x})}*\\frac{2}{x} + c_2\\cos{(2\\ln{x})}*\\frac{2}{x} $$\n",
      "$$ -\\frac{1}{2} = y\\prime(1) = \\frac{1}{2}(c_1+0) + 1(2c_2) $$\n",
      "$$ c_2 = 0 $$\n",
      "\n",
      "Solution of the IVP is:\n",
      "$$ y(x)=-x^{\\frac{1}{2}} \\cos{(2\\ln{x})} $$"
     ]
    },
    {
     "cell_type": "markdown",
     "metadata": {},
     "source": [
      "### Third Order Example\n",
      "$$ x^3y\\prime\\prime\\prime + 5x^2y\\prime\\prime + 7xy\\prime+ 8y = 0 $$\n",
      "$$ y(x)=x^m $$\n",
      "$$ y\\prime(x) = mx^{m-1} $$\n",
      "$$ y\\prime\\prime(x) = m(m-1)x^{m-2} $$\n",
      "$$ y\\prime\\prime\\prime(x) = m(m-1)(m-2)x^{m-3} $$\n",
      "\n",
      "$$ x^m(m^3+2m^2+4m+8) = 0 $$\n",
      "(This is easy to factor, just group the first 2 terms and the last two)\n",
      "$$ m^2(m+2)+4(m+2) = 0 $$\n",
      "$$ (m+2)(m^2+4) = 0 $$\n",
      "\n",
      "$$ m_1 = -2, m_2 = 2i, m_3 = -2i $$\n",
      "\n",
      "So the general solution is:\n",
      "$$ y(x) = c_1x^{-2}+c_2\\cos{(2\\ln{x})}+c_3\\sin{(2\\ln{x})} $$\n",
      "\n",
      "## Example\n",
      "$$ x^2y\\prime\\prime + 3xy\\prime + 3y = 2x^4e^x $$\n",
      "$$ x^2y\\prime\\prime  - 3xy\\prime + 3y = 0 $$\n",
      "\n",
      "$$ y(x)=x^m $$\n",
      "\n",
      "$$ m(m-1)x^m-3mx^m + 3x^m = 0 $$\n",
      "$$ m^2-m-3m+3=0 $$\n",
      "$$ m^2 -3m + 3 = 0 $$\n",
      "Gives us roots:\n",
      "$$ m_1,2 = \\frac{4\\pm\\sqrt{16-12}}{2}=\\frac{4\\pm2}{2} = 3, 1 $$\n",
      "\n",
      "$$ y_c(x)=c_1x+c_2x^3 $$\n",
      "\n",
      "Now we use variation of parameters to get $y_p$:\n",
      "$$ y_p(x) = u_1(x)y_1(x) + u_2(x)y_2(x) $$\n",
      "Where $y_1=x, y_2=x^3$\n",
      "\n",
      "$$ u_1\\prime = \\frac{W_1}{W}, u_2\\prime = \\frac{W_2}{W} $$\n",
      "$$ y\\prime\\prime - \\frac{3}{x}y\\prime + \\frac{3}{x^2}y = 2x^2e^x $$\n",
      "\n",
      "$$ f(X) = 2x^2e^x $$\n",
      "$$ W = \\begin{vmatrix} x & x^3 \\\\\\ 1 & 3x^2 \\end{vmatrix} $$\n",
      "$$ W_1 = \\begin{vmatrix} 0 & x^3 \\\\\\ 2x^2e^x & 3x^2 \\end{vmatrix} $$\n",
      "$$ W_2 = \\begin{vmatrix} x & 0 \\\\\\ 1 & 2x^2e^x \\end{vmatrix} $$\n",
      "\n",
      "$$ u_1\\prime = -x^2 e^x \\Rightarrow Integrate by parts twice \\Rightarrow u_1(x)=-x^2e^x+2xe^x-2e^x $$\n",
      "$$ u_2\\prime = e^ \\Rightarrow u_2(x)=e^x $$\n",
      "\n",
      "$$ y_p(x)=(-2x^2e^x+2xe^x-2e^x)x+e^xx^3 = 2x^2e^x-2xe^x $$\n",
      "\n",
      "Finally:\n",
      "$$ y(x) =  y_c(x)+y_p(x)=c_1x+c_2x^3 + 2x^2e^x - 2xe^x $$"
     ]
    },
    {
     "cell_type": "markdown",
     "metadata": {},
     "source": [
      "## Notice Simliarity?\n",
      "$$ ay\\prime\\prime = by\\prime + cy = 0 $$\n",
      "$$ y(x)=c_1e^{m_1}+c_2e^{m_2x} $$\n",
      "\n",
      "$$ 2x^2y\\prime\\prime + bxy\\prime + cy = 0 $$\n",
      "$$ y(x)=c_1x^{m_1}+c_2x^{m_2} $$\n",
      "\n",
      "$$ e^{\\ln{x}} = x, x > 0 $$\n",
      "$$ y(x) = c_1e^{m_1\\ln{x}} + c_2e^{m_2\\ln{x}} + c_1e^{m_1t}+c_2e^{m_2t} $$\n",
      "\n",
      "**Ex.**\n",
      "$$ x^2y\\prime\\prime - xy\\prime + y = 0, x>0 $$\n",
      "$$ x=e^t, t=\\ln{x} $$\n",
      "(Chain rule fun!)\n",
      "\n",
      "$$ \\frac{dy}{dx} = \\frac{dy}{dt}\\frac{dt}{dx} = \\frac{1}{x}\\frac{dy}{dt} $$\n",
      "$$ \\frac{d^2y}{dx^2} = \\frac{1}{x}\\frac{d}{dx}(\\frac{dy}{dt}) + (-\\frac{1}{x^2})\\frac{dy}{dt} $$\n",
      "\n",
      "What is $ \\frac{d}{dx}\\frac{dy}{dt} $?\n",
      "$$ \\frac{d}{dx}\\frac{dy}{dt} = \\frac{d}{dx}y\\prime(t(x)) = \\frac{dy\\prime}{dx}\\frac{1}{x}=\\frac{d^2y}{dt^2} $$\n",
      "\n",
      "So, $$ \\frac{d^2y}{dx^2} = \\frac{1}{x^2}(\\frac{d^2y}{dt^2}-\\frac{dy}{dt}) $$\n",
      "\n",
      "So we need to sub:\n",
      "$$ x^2y\\prime\\prime - xy\\prime + y = x^2 \\frac{1}{x^2}(\\frac{d^2y}{dt^2}-\\frac{dy}{dy}) - x\\frac{1}{x}\\frac{dy}{dt}t + y = 0 $$\n",
      "$$ \\frac{d^2y}{dt^2}-2\\frac{dy}{dt} + y = 0 $$\n",
      "\n",
      "Hey look! A second order equation with constnat coefficients. We can **solve this!**\n",
      "$$ m^2-2m+1 = 0 $$\n",
      "$$ m_1=m_2=1 $$\n",
      "$$ y_c(t)=c_1e^+c_2te^t $$\n",
      "\n",
      "Do the substitution for $t \\rightarrow x$:\n",
      "$$ y_c(x)=c_1e^{\\ln{x}} + c_2\\ln{x}e^{\\ln{x}} $$\n",
      "$$ y_c(x) = c_1x+c_2x\\ln{x} $$"
     ]
    },
    {
     "cell_type": "markdown",
     "metadata": {},
     "source": [
      "# Homework\n",
      "Pg 168-169\n",
      "You'll see a form for the equations more general: $a(x-x_0)^2y\\prime\\prime + b(x-x_0)y\\prime + cy = 0$... What we did $x_0$ is zero."
     ]
    },
    {
     "cell_type": "code",
     "collapsed": false,
     "input": [],
     "language": "python",
     "metadata": {},
     "outputs": []
    }
   ],
   "metadata": {}
  }
 ]
}