{
 "metadata": {
  "name": "13-Solutions about Ordinary Coordinates"
 },
 "nbformat": 3,
 "nbformat_minor": 0,
 "worksheets": [
  {
   "cells": [
    {
     "cell_type": "markdown",
     "metadata": {},
     "source": [
      "# 6.2 Solutions about Ordinary Coordinates - Math 201\n",
      "### Dr. Florin Diacu (http://www.math.uvic.ca/faculty/diacu/)"
     ]
    },
    {
     "cell_type": "markdown",
     "metadata": {},
     "source": [
      "## NOTE:\n",
      "The textbook has some **huge** mistakes in this section.\n",
      "\n",
      "Ignore how he talks **Singular Points** about $f(x)=\\ln{x}$ is discontinuous, also $g(x)=\\frac{1}{x}$."
     ]
    },
    {
     "cell_type": "markdown",
     "metadata": {},
     "source": [
      "This is (*):\n",
      "$$ a_2(x)y\\prime\\prime + a_1(x)y\\prime + a_0(x)y = 0 $$\n",
      "$ a_0, a_1, a_2 $ are polynomials.\n",
      "\n",
      "## Definition\n",
      "A point $x=x_0$ is called an ordinary point for (*) if it is not a solution of the equation $a_2(x)=0$. If $x_0$ is a solution of $a_2(x)=0$, if is called a singular point.\n",
      "\n",
      "**Ex.**\n",
      "\n",
      "$$ xy\\prime\\prime + (x+1)y\\prime - y = 0 $$\n",
      "$x=0$ is a singular point.\n",
      "\n",
      "Any other $x$ is a regular point.\n",
      "\n",
      "In standard form, the equation becomes\n",
      "$$ y\\prime\\prime + \\frac{x+1}{x}y\\prime - \\frac{1}{x}y = 0 $$\n",
      "Restricted to $(0,\\infty)$ or $(-\\infty,0)$.\n",
      "\n",
      "We are interested in power series solutions about points $x_0\\neq0$"
     ]
    },
    {
     "cell_type": "markdown",
     "metadata": {},
     "source": [
      "## Theorem\n",
      "If $x=x_0$ is an ordinary point of a differential equation with polynomial coefficients, we can always fine two linearly independent solutions in the form of a power series centered at $x_0$, that is\n",
      "$$ y(x) = \\sum_{n=0}^{\\infty}{ c_n(x-x_n)^n } $$\n",
      "A power series solution converges at least on some interval $|x-x_0| \\lt R$, where $R$ is the distance from $x_0$ to the closest singular point.\n",
      "\n",
      "**Ex.**\n",
      "\n",
      "$$ (x^2+1)y\\prime\\prime + xy\\prime + x^3y = 0 $$\n",
      "If we seek a power series solution about $x=0$, it will be convergent in the interval $(-1,1)$ at least. (From theorem)\n",
      "\n",
      "Singular points, roots of\n",
      "$$ x^2+1 = 0 $$\n",
      "$$ x_1=i, x_2=-i $$\n",
      "\n",
      "**Ex.**\n",
      "\n",
      "$$ (x^2-2x+5)y\\prime\\prime + xy\\prime - y = 0 $$\n",
      "\n",
      "$$ x^2-2x+5 = 0 $$\n",
      "$$ x_{1,2} = \\frac{-2\\pm \\sqrt{4-20}}{2} $$\n",
      "$$ x_1 = 1+2i, x_2=1-2i $$\n",
      "\n",
      "And $x=0$, $x=-1$ are our cases.\n",
      "\n",
      "\n",
      "Case (a):\n",
      "$$x=0$$\n",
      "The distance from $0$ to $1\\pm 2i$ is $\\sqrt{5}$.\n",
      "\n",
      "So it's convergent in $(-\\sqrt{5},\\sqrt{5})$.\n",
      "\n",
      "Case(b):\n",
      "$$x=-1$$\n",
      "Distance from $-1$ to $1\\pm 2i$ is $2\\sqrt{2}$. So the series are convergent in $(-1-\\sqrt{2}, -1+2\\sqrt{2})$ at least.\n",
      "\n",
      "### Ex.\n",
      "This is called **Airy's Equation**\n",
      "$$ y\\prime\\prime + xy = 0 $$\n",
      "\n",
      "Lets do it around $x=0$. (The theorem implies that $R\\Rightarrow \\infty$, so convergence is assured in $(-\\infty, \\infty)$.\n",
      "\n",
      "Seeking solutions of the form:\n",
      "$$ y(x) = \\sum_{n=0}^{\\infty}{ c_nx^n } $$\n",
      "$$ y\\prime(x) = \\sum_{n=1}^{\\infty}{ c_n(n)x^{n-1} } $$\n",
      "$$ y\\prime\\prime(x) = \\sum_{n=2}^{\\infty}{ c_n(n)(n-1)x^{n-2} } $$\n",
      "\n",
      "$$ y\\prime\\prime + xy = \\sum_{n=2}^{\\infty}{ c_n(n)(n-1)x^{n-2} } + \\sum_{n=0}^{\\infty}{ c_nx^n } = \\sum_{n=2}^{\\infty}{ c_n(n)(n-1)x^{n-2} } $$\n",
      "\n",
      "As we saw in the last lecture, this is:\n",
      "$$ y\\prime\\prime + xy = 2c_2 + \\sum_{k=1}^{\\infty}{ ((k+1)(k+2)c_{k+2} + c_{k-1})x^k } = 0 $$\n",
      "\n",
      "It follows that:\n",
      "$$ 2c_2 = 0 \\Rightarrow c_2 = 0 $$\n",
      "$$ (k+1)(k+2)c_{k+2}+c_{k-1} = 0 $$\n",
      "Which is our recurrance relation!\n",
      "\n",
      "$$ c_{k=2} = \\frac{c_{k-1}}{(k+1)(k+2)} $$\n",
      "$$ k = 1, 2, ... $$\n",
      "\n",
      "$$ k=1, c_3 = -\\frac{c_0}{2*3} $$\n",
      "$$ k=2, c_4 = -\\frac{c_1}{3*4} $$\n",
      "$$ k=3, c_5 = -\\frac{c_2}{4*5} = 0 $$\n",
      "$$ k=4, c_6 = -\\frac{c_3}{5*6} = \\frac{1}{2*3*5*6}c_0 $$\n",
      "$$ k=5, c_7 = -\\frac{c_4}{6*7} = \\frac{1}{3*4*6*7}c_1 $$\n",
      "$$ k=6, c_8 = -\\frac{c_5}{7*8} = 0 $$\n",
      "$$ k=7, c_9 = -\\frac{c_6}{8*9} = -\\frac{1}{2*3*5*6*8*9}c_0 $$\n",
      "$$ k=8, c_{10} = -\\frac{c_7}{9*10} = -\\frac{1}{3*4*6*7*9*10}c_1 $$\n",
      "$$ k=9, c_{11} = -\\frac{c_8}{10*11} = 0 $$\n",
      "\n",
      "When $k % 3 = 0$, it's $0$.\n",
      "\n",
      "$$ y(x) = c_0 + c_1x + c_2x^2 + c_3x^3 + ... + c_{11}x^{11} + ... $$\n",
      "$$ y(x) = c_0 + c_1x + 0 - \\frac{c_0}{2*3}x^3  - \\frac{c_1}{3*4}x^4 + 0 + \\frac{c_0}{2*3*5*6}x^6 + \\frac{c_1}{3*4*6*7}x^7 + 0 - \\frac{c_0}{2*3*5*6*8*9}x^9 - \\frac{c_1}{3*4*6*7*9*10}x^{10} + 0 + ... $$\n",
      "\n",
      "So take:\n",
      "$$ y_1(x) = 1 - \\frac{1}{2*3}x^3 + \\frac{1}{2*3*5*6}x^6 - \\frac{1}{2*3*5*6*8*9}x^9 + ... = 1 + \\sum_{k=1}^{\\infty}{ \\frac{(-1)^k}{2*3*...(3k-1)(3k)}x^{3k} } $$\n",
      "$$ y_2(x) = x - \\frac{1}{3*4}x^4 + \\frac{3*4*6*7}x^7 - \\frac{1}{3*4*6*7*9*10}x^{10} + ... = x + \\sum_{k=1}^{\\infty}{ \\frac{(-1)^k}{3*4*...(3k)(3k+1)}x^{1+k} } $$"
     ]
    },
    {
     "cell_type": "markdown",
     "metadata": {},
     "source": [
      "### Ex.\n",
      "An example where the coefficients are not polynomials\n",
      "\n",
      "$$ y\\prime\\prime+(\\cos{x})y=0 $$\n",
      "We can find a power series solution $y(x)=\\sum_{n=0}^{\\infty}{ c_nx^n }$ (about $x=0$)\n",
      "\n",
      "$$ y\\prime\\prime+(\\cos{x})y = \\sum_{n=2}^{\\infty}{ n(n-1)c_nx^{n-2} } + (1-\\frac{x^2}{2!}+\\frac{x^4}{4!}-\\frac{x^6}{6!}+...)\\sum_{n=0}^{\\infty}{ c_nx^n } $$\n",
      "$$ = 2c_2 + 6c_3x + 12c_4x^2 + 20c_5x^3 + ... + (1-\\frac{x^2}{2!}+\\frac{x^4}{4!}-...)(c_0 + c_1x + c_2x^2 + c_3x^3 + ... ) $$\n",
      "\n",
      "Group terms by $x$:\n",
      "$$ = c_0+2c_2 + (c_1+6c_3)x + (-\\frac{1}{2}c_0+c_2+12c_4)x^2 + (-\\frac{1}{2}c_1+c_3+20c_5)x^3 + ... = 0 $$\n",
      "\n",
      "So now we can at least compute the first few coefficients of the equation.\n",
      "$$ \\Rightarrow c_0 + 2c_2 = 0 $$\n",
      "$$ \\Rightarrow c_1+ 6c_3 = 0 $$\n",
      "$$ \\Rightarrow -\\frac{1}{2}c_0 + c_2 + 12c_4 = 0 $$\n",
      "$$ \\Rightarrow -\\frac{1}{2}c_1 + c_3 + 20c_5 = 0 $$\n",
      "\n",
      "$$ c_2 = -\\frac{1}{2}c_0 $$\n",
      "$$ c_3 = -\\frac{1}{6}c_1 $$\n",
      "$$ c_4 = \\frac{1}{12}c_0 $$\n",
      "$$ c_3 = \\frac{1}{30}c_1 $$\n",
      "It's natural to have $c_0, c_1$ as constants. Since we have 2 unknowns.\n",
      "\n",
      "$$ y(x) = c_0y_1(x) + c_2y_2(x) $$\n",
      "$$ y_1(x) = 1 - \\frac{1}{2}x_2 + \\frac{1}{12}x^4 $$\n",
      "$$ y_2(x) = x - \\frac{1}{6}x^3 + \\frac{1}{30}x^5 $$\n",
      "\n",
      "Since the coefficient of $y\\prime\\prime$ is $1$, the series are convergent for all $x\\in\\mathbb{R}$."
     ]
    },
    {
     "cell_type": "code",
     "collapsed": false,
     "input": [],
     "language": "python",
     "metadata": {},
     "outputs": []
    }
   ],
   "metadata": {}
  }
 ]
}