{
 "metadata": {
  "name": "18-Operational Properties p2"
 },
 "nbformat": 3,
 "nbformat_minor": 0,
 "worksheets": [
  {
   "cells": [
    {
     "cell_type": "markdown",
     "metadata": {},
     "source": [
      "# 7.4 Operational Properties Part 2 - Math 201\n",
      "### Dr. Florin Diacu (http://www.math.uvic.ca/faculty/diacu/)"
     ]
    },
    {
     "cell_type": "markdown",
     "metadata": {},
     "source": [
      "$$ \\frac{d}{ds}F(s) = \\frac{d}{ds} \\int_0^\\infty{ e^{-st}f(t) dt } = \\int_0^\\infty{ \\frac{\\partial}{\\partial s}[e^{-st}f(t)dt } = -\\int_0^\\infty{ e^{-st}tf(t)dt } = -L\\\\{tf(t)\\\\} $$\n",
      "\n",
      "$$ L\\\\{tf(t)\\\\} = -\\frac{d}{ds}L\\\\{f(t)\\\\} $$\n",
      "$$ L\\\\{t^2f(t)\\\\} = L\\\\{t*tf(t)\\\\} = -\\frac{d}{ds}L\\\\{t f(t)\\\\} = -\\frac{d}{ds}(-\\frac{d}{ds}L\\\\{f(t)\\\\}) = \\frac{d^2}{ds^2}L\\\\{f(t)\\\\} $$"
     ]
    },
    {
     "cell_type": "markdown",
     "metadata": {},
     "source": [
      "# Theorem: Derivatives of transforms\n",
      "$$ F(s) = L\\\\{f(t)\\\\}, n=1,2,3,... $$\n",
      "$$ L\\\\{t^nf(t)\\\\} = (-1)^n \\frac{d^n}{ds^n}F(s) $$\n",
      "\n",
      "### Ex\n",
      "Evaluate\n",
      "$$ L\\\\{t\\sin{kt}\\\\} $$\n",
      "\n",
      "$$ f(t) = \\sin{kt}, f(s)=\\frac{k}{s^2+k^2}, n=1 $$\n",
      "$$ L\\\\{t\\sin{kt}\\\\} = -\\frac{d}{ds}L\\\\{\\sin{kt}\\\\} = - \\frac{d}{ds}(\\frac{k}{s^2+k^2}) = \\frac{2ks}{(s^2+k^2)^2} $$\n",
      "\n",
      "### Ex\n",
      "$$ L\\\\{te^{3t}\\\\} = L\\\\{t\\\\}_{s\\Rightarrow s-3} = \\frac{1}{s^2} \\Rightarrow \\frac{1}{(s-3)^2} $$\n",
      "Another way:\n",
      "$$ L\\\\{te^{3t}\\\\} = -\\frac{d}{ds}L\\\\{e^{3t}\\\\} = -\\frac{d}{ds}\\frac{1}{s^{-3}} = (s-3)^{-2} = \\frac{1}{(s-3)^2} $$\n",
      "\n",
      "### Ex\n",
      "$$ x\\prime\\prime + 16x = \\cos{4t}, x(0)=0, x\\prime(0)=1 $$\n",
      "\n",
      "This is like the motion of a spring (The $\\cos{4t}$ represents a wave, so lets say it's on a ship)\n",
      "\n",
      "$$ X(s) = L\\\\{x(t)\\\\} $$\n",
      "$$ (s^2 + 16)X(s) = 1+ \\frac{s}{x^2+16} $$\n",
      "$$ X(s) = \\frac{1}{s^2+16} + \\frac{s}{(s^2+16)^2} $$\n",
      "\n",
      "From the previous example we know:\n",
      "$$ L^{-1}\\\\{ \\frac{2ks}{(s^2+k^2)^2} \\\\} = t\\sin{kt} $$\n",
      "\n",
      "$ k = 4 $ recall that\n",
      "$$ \\sin{kt} = L^{-1}\\\\{ \\frac{k}{s^2+k^2} \\\\} $$\n",
      "\n",
      "$$ x(t) = \\frac{1}{4}L^{-1}\\\\{ \\frac{4}{s^2+16} \\\\} + \\frac{1}{8}L^{-1}\\\\{ \\frac{8s}{(s^2+16)^2} \\\\} = \\frac{1}{4}\\sin{4t} + \\frac{1}{8}t\\sin{4t} $$"
     ]
    },
    {
     "cell_type": "markdown",
     "metadata": {},
     "source": [
      "# Convolution\n",
      "$f,g$ peicewise continuous functions on $[0,\\infty)$.\n",
      "\n",
      "$$ (f*g)(t) = \\int_0^t{ f(\\tau)g(t-\\tau)d\\tau } $$\n",
      "\n",
      "### Ex\n",
      "$$ e^t * \\sin{t} = \\int_0^t{ e^\\tau \\sin{t-\\tau} d\\tau } $$\n",
      "Compute this using integration by parts.\n",
      "$$ = \\frac{1}{2}(-\\sin{t}-\\cos{t}+e^t) $$\n",
      "\n",
      "## Convolution Commutes\n",
      "$$ \\int_0^t{ f(\\tau)g(t-\\tau)d\\tau } = \\int_0^t{ f(t-\\tau)g(\\tau)d\\tau } $$\n",
      "$$ f*g = g*f $$\n",
      "\n",
      "## Theorem: Convolution Theorem\n",
      "If $f,g$ are pieceiwse continuous on $[0,\\infty)$ and of exponential order.\n",
      "Then:\n",
      "$$ L\\\\{ (f*g)(t) \\\\} = L\\\\{ f(t) \\\\} * L\\\\{ g(t) \\\\} = F(s)G(s) $$\n",
      "\n",
      "This property is crucial as it allows us to solve certain problems.\n",
      "\n",
      "### Ex\n",
      "$$ L\\\\{ \\int_0^t{ e^\\tau\\sin(t-\\tau)d\\tau } \\\\} $$\n",
      "$$ f(t)=e^t, g(t) = \\sin{t} $$\n",
      "$$ L\\\\{ \\int_0^t{ e^\\tau\\sin(t-\\tau)d\\tau } \\\\} = L\\\\{e^t\\\\}L\\\\{\\sin{t}\\\\} = \\frac{1}{s-1}*\\frac{1}{s^2+1} = \\frac{1}{(s-1)(s^2+1) $$\n",
      "\n",
      "## Inverse\n",
      "$$ L^{-1}\\\\{ F(s)G(s) \\\\} = (f*g)(t) $$\n",
      "\n",
      "### Ex\n",
      "$$ L^{-1}\\\\{ \\frac{1}{(s^2+k^2)^2} \\\\} $$\n",
      "$$ F(s) = G(s) = \\frac{1}{s^2+k^2} $$\n",
      "$$ f(t) = g(t) = \\frac{1}{k} L^{-1}\\\\{ \\frac{k}{s^2+k^2} \\\\} = \\frac{1}{k}\\sin{kt} $$\n",
      "\n",
      "$$ L^{-1}\\\\{ \\frac{1}{(s^2+k^2)^2} = \\frac{1}{k^2} \\int_0^t{ \\sin{kt}*\\sin{k(t-\\tau)} d\\tau } $$\n",
      "$$ \\sin{A}\\sin{B} = \\frac{1}{2}[\\cos{A-B}-\\cos{A+B}] $$\n",
      "$$ A = k\\tau, B = k(t-\\tau) $$\n",
      "\n",
      "$$ L^{-1}\\\\{ \\frac{1}{(s^2+k^2)^2} \\\\} = \\frac{1}{2k^2} \\int_0^t{ [\\cos{k(2\\tau-t)}-\\cos{k\\tau}]d\\tau } $$\n",
      "$$ = \\frac{1}{2k^2}[ \\frac{1}{2k} \\sin{k(2\\tau-t)}^0 - \\tau\\cos{kt} ]_0^t = \\frac{\\sin{kt}-kt\\cos{kt}}{2k^3} $$\n",
      "\n",
      "$$ L\\\\{ \\sin{kt} - kt\\cos{kt} \\\\} = \\frac{2k^3}{(s^2+k^2)^2} $$\n",
      "\n",
      "## This follows:\n",
      "$$ g(t) = 1, L\\\\{g(t)\\\\} = G(s) = \\frac{1}{s} $$\n",
      "**IMPORTANT BELOW**\n",
      "$$ L\\\\{ \\int_0^t{ f(\\tau)d\\tau \\\\} = \\frac{F(s)}{s} $$ \n",
      "$$ F(s) = L\\\\{f(t)\\\\} $$\n",
      "**IMPORTANT BELOW**\n",
      "$$ \\int_0^t{ f(\\tau)d\\tau } = L^{-1}\\\\{ \\frac{f(s)}{s} \\\\} $$\n",
      "\n",
      "## Ex\n",
      "$$ f(t) = \\sin{t}, F(s) = \\frac{1}{s^2+1} $$\n",
      "$$ L^{-1}\\\\{ \\frac{1}{s(s^2+1)} \\\\} = L^{-1}\\\\{ \\frac{\\frac{1}{s^2+1}}{s} \\\\} = \\int_0^t{\\sin{\\tau}d\\tau} = 1 - \\cos{t} $$\n",
      "$$ L^{-1}\\\\{ \\frac{1}{s^2(s^2+1)} \\\\} = L^{-1}\\\\{ \\frac{\\frac{1}{s(s^2)+1)}}{s} = \\int_0^t(1-\\cos{\\tau}d\\tau = t-\\sin{t} $$\n",
      "$$ L^{-1}\\\\{ \\frac{1}{s^3(s^2+1)} \\\\} = L^{-1}\\\\{ \\frac{\\frac{1}{s^2(s^2+1)}}{s} = \\int_0^t{\\tau-\\sin{\\tau}d\\tau } = \\frac{1}{2}t^2-1+\\cos{t} $$\n"
     ]
    },
    {
     "cell_type": "markdown",
     "metadata": {},
     "source": [
      "# Voltera's Integral Equation\n",
      "$$ f(t)=g(t)+ \\int_0^t{ f(\\tau)h(t-\\tau)d\\tau } $$\n",
      "$ g,h $ Given.... $f$ unknown....\n",
      "\n",
      "### Ex\n",
      "$$ f(t) = 3t^2 - e^{-t} - \\int_0^t{ f(\\tau)e^{t-\\tau} d\\tau } $$\n",
      "\n",
      "Compare to the theorem:\n",
      "$$ h(t-\\tau) = e^{t-\\tau} \\Rightarrow h(t) = e^t $$\n",
      "$$ L\\\\{e^t\\\\} = \\frac{1}{s-1} $$\n",
      "$$ L\\\\{f(t)\\\\} = F(s) $$\n",
      "$$ F(s) = 3*\\frac{2}{s^3} - \\frac{1}{s+1} - F(s)\\frac{1}{s-1} $$\n",
      "Where $ F(s)\\frac{1}{s-1} $ is the convolution.\n",
      "\n",
      "Now we have an algebraic equation in $F$.\n",
      "$$ F(s) = \\frac{6}{s^3} - \\frac{6}{s^4} + \\frac{1}{s} - \\frac{2}{s+1} $$\n",
      "\n",
      "Now apply the inverse laplace\n",
      "$$ f(t) = 3L^{-1}\\\\{ \\frac{2!}{s^3} \\\\} - L^{-1}\\\\{ \\frac{3!}{s^4} \\\\} + L^{-1}\\\\{ \\frac{1}{s} \\\\} - 2L^{-1}\\\\{ \\frac{1}{s+1} \\\\} = 3t^2 - t^3 +1 - 2e^{-t} $$\n",
      "\n",
      "### Ex (Application for elec engineers)\n",
      "**Kirchhoff's 2nd Law**:\n",
      "$$ L \\frac{di}{dt} , Ri(t) $$\n",
      "$$ \\frac{1}{C} \\int_0^t{ i(\\tau)d\\tau } $$\n",
      "\n",
      "Where $i=$ current, $L,R$ constant.\n",
      "\n",
      "This leads us to a so called integral differential equation\n",
      "$$ L \\frac{di}{dt} + Ri(t) + \\frac{1}{C}\\int_0^t{ i(\\tau)d\\tau } = E(t) $$\n",
      "Here $i$ occurs as a derivative, an integral, and a multiple.\n"
     ]
    },
    {
     "cell_type": "code",
     "collapsed": false,
     "input": [],
     "language": "python",
     "metadata": {},
     "outputs": []
    }
   ],
   "metadata": {}
  }
 ]
}