{
 "metadata": {
  "name": "Assignment 1"
 },
 "nbformat": 3,
 "nbformat_minor": 0,
 "worksheets": [
  {
   "cells": [
    {
     "cell_type": "markdown",
     "metadata": {},
     "source": [
      "# Assignment 1 - Math 201\n",
      "### Professor: Dr. Florin Diacu\n",
      "### Student: Andrew Hobden (V00788452)"
     ]
    },
    {
     "cell_type": "markdown",
     "metadata": {},
     "source": [
      "# Question 1\n",
      "Solve the Equation: $x^\\prime = x^2 -4$\n",
      "\n",
      "### Separating Variables:\n",
      "$$ \\begin{matrix} g(x) = x^2-4 \\\\\\ h(t) = 1 \\end{matrix} \\Rightarrow\n",
      "\\frac{dx}{dy} = g(x)*h(t) $$\n",
      "\n",
      "### Integrating:\n",
      "$$ \\int{\\frac{dx}{x^2-4}} = \\int{1 dt} $$\n",
      "\n",
      "Via Partial Fractions:\n",
      "$$ \\frac{1}{x^2-4} = \\frac{A(x-2)+B(x+2)}{(x+2)(x-2)} $$\n",
      "$$ A = -\\frac{1}{4}, B = \\frac{1}{4} $$\n",
      "\n",
      "Substituting:\n",
      "$$ \\int{\\frac{-\\frac{1}{4}}{x+2}dx} + \\int{\\frac{\\frac{1}{4}}{x-2}dx} = \\int{1dt} $$\n",
      "\n",
      "The Implicit Solution:\n",
      "$$ -\\frac{1}{4}\\ln{|x+2|} + \\frac{1}{4}\\ln{|x-2|} = t+c $$\n",
      "\n",
      "### Solving for $x$:\n",
      "Via log rules:\n",
      "$$ \\ln{\\frac{x-2}{x+2}}=4(t+c) $$\n",
      "$$ \\frac{x-2}{x+2}= e^{4t+4c} $$\n",
      "$$ x-2 = xe^{4t+4c} + 2e^{4t+4c} $$\n",
      "$$ x = \\frac{2e^{4t+4c}+2}{1-e^{4t+4c}} $$\n",
      "\n",
      "Which simplifies to our **explicit solution**:\n",
      "$$ x = \\frac{-2(e^{4t+4c} +1)}{e^{4t+4c}-1} $$\n",
      "\n",
      "However since $e^{4c}$ is simply a constant, we can simplify further to:\n",
      "$$ x = \\frac{-2(e^{4t}*k+1)}{e^{4t}*k-1} $$\n",
      "\n",
      "### Singular Solutions\n",
      "**Already accounted for** in the general solution.\n",
      "$$ x=2 \\Rightarrow x^\\prime = 2^2 - 4 = 0 $$\n",
      "$$ \\gamma(t) = 2, \\gamma : \\mathbb{R} \\rightarrow \\mathbb{R} $$\n",
      "\n",
      "**Required singular solution**.\n",
      "$$ x=-2 \\Rightarrow x^\\prime=(-2)^2-4=0 $$\n",
      "$$ \\gamma(t)=-2, \\gamma : \\mathbb{R} \\rightarrow \\mathbb{R} $$"
     ]
    },
    {
     "cell_type": "markdown",
     "metadata": {},
     "source": [
      "# Question 2\n",
      "What is the half-life of Krypton 85, knowing that it's decay rate is 6.3% per year?\n",
      "$$ k = \\frac{-6.3}{100} = -0.063 $$\n",
      "$$ C = 1 $$\n",
      "$$ x(t) = .5 $$\n",
      "\n",
      "The general solution: $ x(t) = Ce^{kt} $\n",
      "\n",
      "### Substituting:\n",
      "$$ 0.5 = 1e^{-0.063t} $$\n",
      "\n",
      "### Solving:\n",
      "$$ \\frac{\\ln{0.5}}{-0.063} = t $$\n",
      "$$ t = 11.0023 $$\n",
      "\n",
      "$\\therefore$ The half life is 11.0023 years."
     ]
    },
    {
     "cell_type": "markdown",
     "metadata": {},
     "source": [
      "# Question 3\n",
      "Solve the initial value problem: $ y^\\prime = [(t-1)y]^{-\\frac{1}{3}} $\n",
      "\n",
      "When $ y(0)=1 $.\n",
      "\n",
      "Expanding:\n",
      "$$ y^\\prime = (t-1)^{-\\frac{1}{3}}y^{-\\frac{1}{3}} $$\n",
      "\n",
      "### Separating Variables:\n",
      "$$ \\begin{matrix} g(y) = y^{-\\frac{1}{3}} \\\\\\ h(t)=(t-1)^{-\\frac{1}{3}} \\end{matrix}\n",
      "\\Rightarrow \\frac{dy}{g(y)}=h(t)dt\n",
      "$$\n",
      "\n",
      "### Integrating:\n",
      "$$ \\int{\\frac{dy}{y^{\\frac{1}{3}}}} = \\int{\\frac{1}{(t-1)^{\\frac{1}{3}}} dt} $$\n",
      "\n",
      "The implicit solution:\n",
      "$$ \\frac{3}{4}y^{\\frac{4}{3}} = \\frac{3}{2}(t-1)^{\\frac{2}{3}} +c $$\n",
      "\n",
      "### Solving for $y$:\n",
      "$$ y^{\\frac{4}{3}} = 2(t-1)^{\\frac{2}{3}} + c $$\n",
      "\n",
      "The explicit solution:\n",
      "$$ y = [2(t-1)^{\\frac{2}{3}}+c]^{\\frac{3}{4}} $$\n",
      "\n",
      "### Finding the $c$:\n",
      "Using the initial value: $y(0)=1$\n",
      "\n",
      "$$ y(0) = 1 = [2(0-1)^{\\frac{2}{3}} + c]^{\\frac{3}{4}} $$\n",
      "\n",
      "Solving for $c$:\n",
      "$$ 1 = [2(-1)^{\\frac{2}{3}} + c]^{\\frac{3}{4}} $$\n",
      "$$ c = 1^{\\frac{4}{3}} - 2(-1)^{\\frac{2}{3}} $$\n",
      "$$ c = 1-2(1) = -1 $$\n",
      "\n",
      "### Substituting Back\n",
      "$$ y=(2(t-1)^{\\frac{2}{3}}-1)^{\\frac{3}{4}} $$"
     ]
    },
    {
     "cell_type": "markdown",
     "metadata": {},
     "source": [
      "# Question 4\n",
      "Solve the equation $x^\\prime = tx + 6te^{-t^2}$\n",
      "\n",
      "Noting that this is a linear non-homogeneous equation.\n",
      "$$ \\begin{matrix} F(t)=t \\\\\\ g(t)=6te^{-t^2} \\end{matrix}\n",
      "\\Rightarrow  x^\\prime = F(t)x+g(t) $$\n",
      "\n",
      "### Considering $x^\\prime = F(t)x$:\n",
      "$$ \\frac{dx}{dt} = f(t)x = tx $$\n",
      "$$ x = ce^{\\frac{1}{2}t^2} $$\n",
      "\n",
      "Making $c$ a variable:\n",
      "$$ x(t) = c(t)e^{\\frac{1}{2}t^2} $$\n",
      "\n",
      "$$ x^\\prime(t) = c^\\prime(t)e^{\\frac{1}{2}t^2} + tc(t)e^{\\frac{1}{2}t^2} $$\n",
      "\n",
      "### Substituting Back:\n",
      "$$ t(c(t)e^{\\frac{1}{2}t^2}) + 6te^{-t^2} = c^\\prime(t)e^{\\frac{1}{2}t^2} + tc(t)e^{\\frac{1}{2}t^2} $$\n",
      "\n",
      "Noting how the terms containing $c(t)$ cancel out:\n",
      "$$ 6te^{-t^2} = c^\\prime(t)e^{\\frac{1}{2}t^2} $$\n",
      "\n",
      "Solving for $c^\\prime(t)$:\n",
      "$$ c^\\prime(t)=6te^{-t^2}e^{-\\frac{1}{2}t^2} $$\n",
      "\n",
      "Noting that $ 6te^{-t^2} = g(t) $ and $ (-\\frac{1}{2}t) = \\phi $:\n",
      "$$ c(t) = \\int{g(t)e^{\\phi t}dt} $$\n",
      "$$ c(t) = \\int{6te^{-t^2}e^{-\\frac{1}{2}t^2}dt} $$\n",
      "$$ c(t) = -2e^{-\\frac{3}{2}t^2} +k $$\n",
      "\n",
      "### Substituting $c(t)$:\n",
      "$$ x=(-2e^{-\\frac{3}{2}t^2} +k)e^{\\frac{1}{2}t^2} $$"
     ]
    },
    {
     "cell_type": "markdown",
     "metadata": {},
     "source": [
      "# Question 5\n",
      "Solve the initial value problem: $r^\\prime = [\\cot{2\\phi}]r-\\cos{2\\phi}$\n",
      "\n",
      "When $r(\\frac{\\pi}{4})=0$.\n",
      "\n",
      "Noting that this is a linear non-homogeneous equation.\n",
      "$$ \\begin{matrix} F(\\phi)=\\cot{2\\phi} \\\\\\ g(\\phi)=\\cos{2\\phi} \\end{matrix}\n",
      "\\Rightarrow  r^\\prime = F(\\phi)r+g(\\phi) $$\n",
      "\n",
      "### Considering $r^\\prime = F(\\phi)r$:\n",
      "$$ \\frac{dr}{d\\phi} = F(\\phi)r = \\cot{2\\phi}r $$\n",
      "$$ \\int{\\frac{dr}{r}} = \\int{\\cot{2\\phi} d\\phi} $$\n",
      "$$ r = ce^{\\frac{1}{2}\\ln{\\sin{2\\phi}}} $$\n",
      "$$ r = c\\sin^{\\frac{1}{2}}{(2\\phi)} $$\n",
      "\n",
      "Making $c$ a variable:\n",
      "$$ r(\\phi)=c(\\phi)\\sin^{\\frac{1}{2}}{2\\phi} $$\n",
      "$$ r^\\prime(\\phi) = c^\\prime(\\phi)\\sin^{\\frac{1}{2}}{(2\\phi)} + c(\\phi)\\sin^{-\\frac{1}{2}}{(2\\phi)}*(-\\frac{1}{2})(-2\\cos{(2\\phi)}) $$\n",
      "Simplifying:\n",
      "$$ r^\\prime(\\phi) = c^\\prime(\\phi)\\sin^{\\frac{1}{2}}{(2\\phi)}+\\frac{\\cos{(2\\phi)}c(\\phi)}{\\sin^{\\frac{1}{2}}{(2\\phi)}} $$\n",
      "\n",
      "### Substituting Back\n",
      "$$ F(\\phi)r+g(\\phi)=r^\\prime $$\n",
      "$$ c(\\phi)\\cot{(2\\phi)}\\sin^\\frac{1}{2}{(2\\phi)}-\\cos{(2\\phi)}  =  c^\\prime(\\phi)\\sin^\\frac{1}{2}{(2\\phi)}+ \\frac{\\cos{(2\\phi)}c(\\phi)}{\\sin^\\frac{1}{2}{(2\\phi)}} $$\n",
      "\n",
      "Observing how terms containing $c(\\phi)$ cancel out:\n",
      "$$ -\\cos{(2\\phi)} = c^\\prime(\\phi)\\sin^\\frac{1}{2}{(2\\phi)} $$\n",
      "\n",
      "Solving for $c^\\prime(\\phi)$:\n",
      "$$ c^\\prime(\\phi)=\\frac{-\\cos{(2\\phi)}}{\\sin^\\frac{1}{2}{2\\phi}} $$\n",
      "\n",
      "Integrating to find $ c(\\phi) $:\n",
      "$$ c(\\phi)=-\\sqrt{\\sin{2\\phi}} + k $$\n",
      "\n",
      "### Substituting $c(\\phi)$:\n",
      "$$ r = (-\\sqrt{\\sin{2\\phi}} + k)\\sin^{\\frac{1}{2}}{(2\\phi)} $$\n",
      "\n",
      "### Finding $k$:\n",
      "$$ r(\\frac{\\pi}{4})= 0 = (\\sqrt{\\sin{(2\\frac{\\pi}{4}})} + k)\\sin^{\\frac{1}{2}}{(2\\frac{\\pi}{4})} $$\n",
      "$$ k = 1 $$\n",
      "\n",
      "Giving us the **solution**:\n",
      "$$ r = (-\\sqrt{\\sin{2\\phi}} +1)\\sin^{\\frac{1}{2}}{(2\\phi)} $$\n",
      "\n",
      "<!--\n",
      "**(I'm noting that there are more steps to be done here, but this doesn't look anything like the general solution.)**\n",
      "\n",
      "### A Solution\n",
      "Noting that $ r(\\frac{\\pi}{4})=0 $:\n",
      "$$ 0 = c * \\sin^{\\frac{1}{2}}{(2*\\frac{\\pi}{4})} $$\n",
      "$$ c = 0 $$\n",
      "\n",
      "Which implies that\n",
      "$$ r = (0)\\sin^{\\frac{1}{2}}{(2\\phi)} $$\n",
      "$$ r = 0 $$\n",
      "-->"
     ]
    }
   ],
   "metadata": {}
  }
 ]
}