{
 "metadata": {
  "name": "Assignment 2"
 },
 "nbformat": 3,
 "nbformat_minor": 0,
 "worksheets": [
  {
   "cells": [
    {
     "cell_type": "markdown",
     "metadata": {},
     "source": [
      "# Assignment 2 - Math 201\n",
      "### Professor: Dr. Florin Diacu\n",
      "### Student: Andrew Hobden (V00788452)"
     ]
    },
    {
     "cell_type": "markdown",
     "metadata": {},
     "source": [
      "# Question 1\n",
      "Show that $y_1(x)=e^x$ is a solution of the equation\n",
      "$$ y^{\\prime\\prime}-4y^{\\prime}+3y = 0 $$\n",
      "\n",
      "Use the Reduction Method to find a second, linearly independent, solution.\n",
      "\n",
      "## Answer\n",
      "Assuming a solution of the form $y(x)=e^{mx}$.\n",
      "$$ (m^2 - 4m + 3)e^{mx} = 0 $$\n",
      "Since $e^{mx}$ is never 0 we will only consider $m^2 - 4m +3=0$.\n",
      "\n",
      "$$ (m-1)(m-3)=0 $$\n",
      "Therefore $ m_1 = 1, m_2 = 3 $.\n",
      "\n",
      "Using $m_1$, our solution for $y_1(x)=e^{x}$, **thus is it a solution of the equation**.\n",
      "\n",
      "Using Reduction to find a second, linearly independent solution:\n",
      "$$ y^{\\prime\\prime}-4y^{\\prime}+3y=0, y_1=e^x $$\n",
      "Since $y_2$ must be linearly independent, it must be of the form $y_2=u(x)y_1(x)$.\n",
      "$$ y_2=u(x)y_1(x) $$\n",
      "$$ y_2^{\\prime}= u^{\\prime}(x)y_1(x)+u(x)y_1^{\\prime}(x) $$\n",
      "$$ y_2^{\\prime\\prime}= u^{\\prime\\prime}(x)y_1(x) + u^{\\prime}(x)y_1^{\\prime}(x) + u^{\\prime}(x)y_1^{\\prime}(x)+u(x)y^{\\prime\\prime}(x) $$\n",
      "\n",
      "**Note**: We will simpily state $u, y_1, u^{\\prime}$ etc from now on for simplicity.\n",
      "\n",
      "Substituting into the original equation and grouping by $u, u^{\\prime}$, and $u^{\\prime\\prime}$:\n",
      "$$ u^{\\prime\\prime}y_1 + u^{\\prime}(2y^{\\prime}-4y_1) + u(y^{\\prime\\prime}-4y_1^{\\prime}+3) = 0 $$\n",
      "Noting here that as previously stated, $y^{\\prime\\prime}-4y_1^{\\prime}+3 = 0$.\n",
      "\n",
      "We'll set $v = u^{\\prime}$ and $v^{\\prime}=u^{\\prime\\prime}$.\n",
      "$$ v^{\\prime}y_1 = -v(2y_1^{\\prime}-4y_1) $$\n",
      "$$ \\frac{v^{\\prime}}{v} = \\frac{ -(2y_1^\\prime - 4y_1) }{ y_1 } = \\frac{ -2y_1^\\prime }{ y_1 } + 4 $$\n",
      "\n",
      "Solving as a seperable equation:\n",
      "$$ \\ln{v} = -2 \\int{ \\frac{ y_1^\\prime }{ y_1 } }dx + 4\\int{}dx = -2\\ln{y_1}+4x $$\n",
      "Solving for $v$:\n",
      "$$ v = e^{-2x+4x} = e^{2x} $$\n",
      "\n",
      "Getting back to $u$:\n",
      "$$ u = \\int{v}dx = \\int{e^{2x}}dx = \\frac{e^{2x}}{2} $$\n",
      "\n",
      "Recalling that $y_2(x)=u(x)y_1(x)$:\n",
      "$$ y_2(x) = \\frac{e^{2x}}{2}e^{x} = \\frac{1}{2}e^{3x} $$\n",
      "\n",
      "**Which is our second solution.**"
     ]
    },
    {
     "cell_type": "markdown",
     "metadata": {},
     "source": [
      "# Question 2\n",
      "Find the general solution of the equation\n",
      "$$ 2y^{\\prime\\prime\\prime}+7y^{\\prime\\prime}+4y^{\\prime}-4y=0 $$\n",
      "\n",
      "### Answer\n",
      "Assuming $y(x)=e^{mx}$.\n",
      "\n",
      "$$ 2m^3 + 7m^2 + 4m - 4 = 0 $$\n",
      "$$ (m+2)^2(2m-1) = 0 $$\n",
      "$$ m_1 = m_2 = -2 $$\n",
      "$$ m_3 = \\frac{1}{2} $$\n",
      "\n",
      "$$ c_1e^{-2x} + c_2xe^{-2x} + c_3e^{\\frac{1}{2}x} = 0 $$"
     ]
    },
    {
     "cell_type": "markdown",
     "metadata": {},
     "source": [
      "# Question 3\n",
      "Use the method of undetermined coefficients to solve the equation\n",
      "$$ y^{\\prime\\prime}-y = \\cosh{x} $$\n",
      "\n",
      "### Answer\n",
      "$$ y = y_c + y_p $$\n",
      "\n",
      "**Finding $y_c$:**\n",
      "\n",
      "Assuming $y(x)$ is of the form $y(x)=e^{mx}$.\n",
      "$$ m^2-1=0 $$\n",
      "$$ m_1 = 1, m_2 = -1 $$\n",
      "\n",
      "$$ y_c = c_1e^x + c_2e^{-x} $$\n",
      "\n",
      "**Finding $y_p$:**\n",
      "\n",
      "Noting: $\\cosh{x} = \\frac{e^{-x}+e^{x}}{2} $\n",
      "$$ y_p = \\frac{A}{2}e^{-x} + \\frac{B}{2}e^{x} $$\n",
      "However we will have duplication! Fix it:\n",
      "$$ y_p = \\frac{A}{2}xe^{-x} + \\frac{B}{2}xe^{x} $$\n",
      "\n",
      "Substituting $y_p$ and $y_p^{\\prime\\prime}$ into the original equation.\n",
      "$$ -\\frac{A}{2}e^{-x} - \\frac{A}{2}e^{-x} + \\frac{A}{2}xe^{-x} + \\frac{B}{2}e^x + \\frac{B}{2}e^x + \\frac{B}{2}xe^x - \\frac{A}{2}xe^{-x} - \\frac{B}{2}xe^x = \\frac{e^{-x}}{2}+ \\frac{e^x}{2} $$\n",
      "$$ -Ae^{-x} + Be^{x} = \\frac{1}{2}e^{-x} + \\frac{1}{2}e^x $$\n",
      "\n",
      "Therefore $A=-\\frac{1}{2}$, $B=\\frac{1}{2}$.\n",
      "\n",
      "So, $y$ is:\n",
      "$$y = y_c + y_p$$\n",
      "$$ y = c_1e^{x}+c_2e^{-x}-\\frac{1}{4}xe^{-x}+\\frac{1}{4}xe^{x} $$\n",
      "<!-- Screwed this up! \n",
      "Assuming $y(x)$ is of the form $y(x)=e^{mx}$.\n",
      "$$ m^2-1=0 $$\n",
      "$$ m = \\sqrt{1} = 1 $$\n",
      "\n",
      "We have real, repeated roots, so $y_c$ of the form $ y_c = c_1e^x+c_2xe^x $\n",
      "\n",
      "**Finding $y_p$ via undetermined coefficients:**\n",
      "\n",
      "Noting that  $\\cosh{x}=\\frac{e^{-x}+e^{x}}{2}$, we'll seek a solution of the form:\n",
      "$$ \\frac{A}{2}e^{-x} +  \\frac{B}{2}e^x $$\n",
      "\n",
      "However since $e^{x}$ already exists within our solution we'll need to make it linearly independent:\n",
      "$$ y_p = \\frac{A}{2}e^{-x} +  \\frac{B}{2}x^2e^x $$\n",
      "$$ y_p^{\\prime} = -\\frac{A}{2}e^{-x} + \\frac{B}{2}xe^{x} + \\frac{B}{2}x^2e^{x} $$\n",
      "$$ y_p^{\\prime\\prime} = \\frac{A}{2}e^{-x} + \\frac{B}{2}e^{x} + \\frac{B}{2}xe^{x} + \\frac{B}{2}xe^{x} + \\frac{B}{2}x^2e^x $$\n",
      "\n",
      "Substituting back into the original equation:\n",
      "$$ \\frac{A}{2}e^{-x} + \\frac{B}{2}xe^{x} + \\frac{B}{2}xe^{x} + \\frac{B}{2}xe^{x} + \\frac{B}{2}x^2e^{x} - \\frac{A}{2}e^{-x} - \\frac{B}{2}x^2e^x = \\frac{e^{-x}+e^{x}}{2} $$\n",
      "$$ \\frac{B}{2}e^{x}+Bxe^{x} = \\frac{e^{-x}+e^x}{2} $$\n",
      "$$ \\frac{B}{2}e^x + Bxe^x = \\frac{e^{-x}+e^{x}}{2} $$\n",
      "$$ B+2Bx = e^{-x} $$\n",
      "\n",
      "Therefore $B = \\frac{e^{-x}}{1+2x}$.\n",
      "Since the $A$'s cancelled, we just choose something convienent since it can be anything, so $A=1$.\n",
      "\n",
      "**The solution:**\n",
      "\n",
      "$$ y = y_c + y_p $$\n",
      "$$ y = c_1e^x + c_2xe^x + \\frac{1}{2}e^{-x} + \\frac{e^{-x}}{2(1+2x)}x^2e^x $$\n",
      "/-->\n"
     ]
    },
    {
     "cell_type": "markdown",
     "metadata": {},
     "source": [
      "# Question 4\n",
      "Solve the equation\n",
      "$$ y^{\\prime\\prime\\prime}+y^{\\prime} = \\tan{x} $$\n",
      "\n",
      "### Answer\n",
      "It makes sense in this problem to do a substitution:\n",
      "$$ y^\\prime = u $$\n",
      "$$ \\therefore u^{\\prime\\prime}+u = \\tan{x} $$\n",
      "\n",
      "**Finding $u_c$:**\n",
      "$$ m^2 + 1 = 0 $$\n",
      "$$ m = \\pm i $$\n",
      "\n",
      "Therefore $ u_c = c_1\\sin{x}+c_2\\cos{x} $.\n",
      "\n",
      "**Finding $u_p$:**\n",
      "$$ W(\\cos{x},\\sin{x}) = \\begin{vmatrix} \\cos{x} & \\sin{x} \\\\\\ -\\sin{x} & \\cos{x} \\end{vmatrix} = \\cos^2{x} + \\sin^2{x} = 1 $$\n",
      "$$ W_1 = \\begin{vmatrix} 0 & \\sin{x} \\\\\\ \\tan{x} & \\cos{x} \\end{vmatrix} = -\\sin{x}\\tan{x} $$\n",
      "$$ W_2 = \\begin{vmatrix} \\cos{x} & 0 \\\\\\ -\\sin{x} & \\tan{x} \\end{vmatrix} = \\cos{x}\\tan{x} $$\n",
      "\n",
      "$$ c_1^\\prime = \\frac{W_1}{W} = -\\sin{x}\\tan{x} $$\n",
      "$$ c_2^\\prime = \\frac{W_2}{W} = \\sin{x} $$\n",
      "\n",
      "$$ c_1 = \\int{c_1^\\prime}dx = \\log{ \\cos{ \\frac{x}{2} } - \\sin{ \\frac{x}{2} } } - \\log{ \\cos{ \\frac{x}{2} } + \\sin{ \\frac{x}{2} } } + \\sin{x} $$\n",
      "$$ c_2 = \\int{c_2^\\prime}dx = -\\cos{x} $$\n",
      "\n",
      "Therefore our $u_p$ simplified is:\n",
      "$$ u_p = \\cos{x}\\log{ \\frac{ \\cos{ \\frac{x}{2} } - \\sin{ \\frac{x}{2} } }{ \\cos{ \\frac{x}{2} } + \\sin{ \\frac{x}{2} } } } $$\n",
      "\n",
      "**Finding $y$:**\n",
      "\n",
      "$$ y^\\prime = u = c_1\\sin{x} + c_2\\cos{x} + \\cos{x}\\log{ \\frac{ \\cos{ \\frac{x}{2} } - \\sin{ \\frac{x}{2} } }{ \\cos{ \\frac{x}{2} } + \\sin{ \\frac{x}{2} } } } $$\n",
      "\n",
      "$$ y = -c_1\\cos{x} + c_2\\sin{x} + \\sin{x}\\log{( \\frac{ \\cos{ \\frac{x}{2} } - \\sin{ \\frac{x}{2} } }{ \\cos{ \\frac{x}{2} } + \\sin{ \\frac{x}{2} } } )} - \\log{( \\cos{ \\frac{x}{2} } - \\sin{ \\frac{x}{2} } )} - \\log{( \\cos{ \\frac{x}{2} } + \\sin{ \\frac{x}{2} } )} + c_3 $$"
     ]
    },
    {
     "cell_type": "markdown",
     "metadata": {},
     "source": [
      "# Question 5\n",
      "Solve the initial value problem\n",
      "$$ x^2 y^{\\prime\\prime} + xy^{\\prime} + y = 0, y(1)=1, y^{\\prime}(1)=2 $$\n",
      "\n",
      "### Answer\n",
      "Using Chachy-Euler.\n",
      "\n",
      "Assuming $y(x)$ is of the form:\n",
      "$$ y(x) = x^m $$\n",
      "$$ y^\\prime(x) = mx^{m-1} $$\n",
      "$$ y^{\\prime\\prime}(x) = m(m-1)x^{m-2} $$\n",
      "\n",
      "Substituting back:\n",
      "$$ x^2m(m-1)x^{m-2} + xmx^{m-1} + x^m = 0 $$\n",
      "$$ m(m-1)+m+1 = 0 $$\n",
      "$$ (m^2 + 1) = 0 $$\n",
      "$$ m_{1,2} = \\pm i $$\n",
      "\n",
      "Using the general solution for complex conjugates:\n",
      "$$ y(x)=c_1x^\\alpha \\cos{(\\beta\\ln{x})}+c_2x^\\alpha \\sin{(\\beta \\ln{x})} $$\n",
      "\n",
      "Gives us our **solution**:\n",
      "$$ y = c_1\\cos{(\\ln{x})} + c_2\\sin{(\\ln{x})} $$\n",
      "We also need it's derivative for the IVP.\n",
      "$$ y^\\prime = \\frac{-c_1\\sin{(\\ln{1})}}{x} + \\frac{c_2\\cos{(\\ln{x})}}{x} $$\n",
      "\n",
      "**Solving the IVP:**\n",
      "$$ y(1) = 1 = c_1\\cos{(\\ln{1})} + c_2 \\sin{(\\ln{1})} $$\n",
      "$$ c_1 = 1 $$\n",
      "\n",
      "$$ y^\\prime (1) = -c_1\\sin{(\\ln{1})} + c_2\\cos{(\\ln{1})} $$\n",
      "$$ c_2 = 1 $$\n",
      "\n",
      "**Finally:**\n",
      "$$ y = \\cos{(\\ln{x})} + \\sin{(\\ln{x})} $$"
     ]
    },
    {
     "cell_type": "code",
     "collapsed": false,
     "input": [],
     "language": "python",
     "metadata": {},
     "outputs": []
    }
   ],
   "metadata": {}
  }
 ]
}